Complete simple proof for tuple except for `RemoveVersions`

src/program_proof/mvcc/tuple_proof.v
@@ -19,18 +19,6 @@ Definition own_tuple (tuple_ptr : loc) (latch : val) : iProp Σ :=
     "Htidwr" ∷ tuple_ptr ↦[Tuple :: "tidwr"] #tidwr ∗
     "Hvers" ∷ tuple_ptr ↦[Tuple :: "vers"] (to_val vers) ∗
     "HversL" ∷ slice.is_slice vers (structTy Version) 1 (ver_to_val <$> versL) ∗
-    (* "HversL" ∷ typed_slice.is_slice vers (structTy Version) 1 versL ∗ *)
-    (* "HversL" ∷ (slice.is_slice vers (structTy Version) 1 (list.untyped versL)) ∗ *)
-    (* "HversL" ∷ (is_slice vers (structTy Version) 1 versL) ∗ *)
-    "%HversLen" ∷ ⌜length versL = int.nat vers.(Slice.sz)⌝ ∗
-    (* Below makes "closing" a bit hard.
-    "Hver" ∷ ([∗ list] k ↦ v ∈ versL,
-               (vers.(Slice.ptr) +ₗ Z.of_nat k) ↦[struct.t Version] (ver_to_val v)) ∗
-    *)
-    "Hver" ∷ ([∗ list] k ↦ v ∈ versL,
-               "Hbegin" ∷ (vers.(Slice.ptr) +ₗ Z.of_nat k) ↦[Version :: "begin"] (to_val v.1.1) ∗
-               "Hend" ∷ (vers.(Slice.ptr) +ₗ Z.of_nat k) ↦[Version :: "end"] (to_val v.1.2) ∗
-               "Hval" ∷ (vers.(Slice.ptr) +ₗ Z.of_nat k) ↦[Version :: "val"] (to_val v.2)) ∗
     "_" ∷ True.
 
 Definition is_tuple (tuple_ptr : loc) : iProp Σ :=
@@ -40,6 +28,196 @@ Definition is_tuple (tuple_ptr : loc) : iProp Σ :=
     "#Hrcond" ∷ readonly (tuple_ptr ↦[Tuple :: "rcond"] #rcond) ∗
     "#HrcondC" ∷ is_cond rcond latch ∗
     "_" ∷ True.
+
+(*****************************************************************)
+(* func (tuple *Tuple) AppendVersion(tid uint64, val uint64)     *)
+(*****************************************************************)
+Theorem wp_tuple__AppendVersion tuple_ptr (tid : u64) (val : u64) :
+  is_tuple tuple_ptr -∗
+  {{{ True }}}
+    Tuple__AppendVersion #tuple_ptr #tid #val
+  {{{ b, RET #b; True }}}.
+Proof.
+  iIntros "#Htuple !#" (Φ) "_ HΦ".
+  iNamed "Htuple".
+  unfold Tuple__AppendVersion.
+
+  (***********************************************************)
+  (* tuple.latch.Lock()                                      *)
+  (***********************************************************)
+  wp_pures.
+  wp_loadField.
+  wp_apply (acquire_spec with "Hlock").
+  iIntros "[Hlocked Hown]".
+  iNamed "Hown".
+  wp_pures.
+
+  (***********************************************************)
+  (* if len(tuple.vers) > 0 {                                *)
+  (*   idx := len(tuple.vers) - 1                            *)
+  (*   verPrevRef := &tuple.vers[idx]                        *)
+  (*   verPrevRef.end = tid                                  *)
+  (* }                                                       *)
+  (***********************************************************)
+  wp_loadField.
+  wp_apply wp_slice_len.
+  wp_if_destruct.
+  { (* `vers` not empty *)
+    wp_loadField.
+    wp_apply wp_slice_len.
+    wp_pures.
+    wp_loadField.
+    wp_lam.
+    wp_pures.
+    wp_apply wp_slice_len.
+    
+    wp_if_destruct; last first.
+    { (* prove in-bound *)
+      exfalso.
+      destruct (bool_decide (int.Z vers.(Slice.sz) = int.Z 0)) eqn:E.
+      - apply bool_decide_eq_true in E. lia.
+      - apply bool_decide_eq_false in E.
+        destruct Heqb0.
+        apply word.decrement_nonzero_lt. done.
+    }
+    wp_apply wp_slice_ptr.
+    wp_pures.
+    iDestruct (slice.is_slice_small_acc with "HversL") as "[HversL HversL_close]".
+    rewrite /slice.is_slice_small.
+    iDestruct "HversL" as "[HversA %HversLen]".
+    (* Below we try to prove the last element of `versL` contains something. *)
+    assert (HversLenLast : ((int.nat (word.sub vers.(Slice.sz) (U64 1))) < length versL)%nat).
+    (* Set Printing Coercions. *)
+    { rewrite fmap_length in HversLen. rewrite HversLen. word. }
+    apply list_lookup_lt in HversLenLast as [x Hsome].
+    iDestruct (update_array with "HversA") as "[Hver HversA]".
+    (* Better proof? *)
+    { rewrite list_lookup_fmap.
+      instantiate (1:=ver_to_val x).
+      instantiate (1:=int.nat (word.sub vers.(Slice.sz) 1)).
+      rewrite Hsome.
+      auto.
+    }
+    iDestruct (struct_fields_split with "Hver") as "Hver".
+    iNamed "Hver".
+    wp_apply (wp_storeField with "[end]"); first auto.
+    { iNext.
+      (* Set Printing Coercions. *)
+      rewrite u64_Z_through_nat.
+      iFrame.
+    }
+    iIntros "end".
+    (* Close things. Better proof? *)
+    remember (vers.(Slice.ptr) +ₗ[struct.t Version] int.nat (word.sub vers.(Slice.sz) 1)) as verLastR.
+    remember (x.1.1, tid, x.2) as verLast.
+    iAssert (verLastR ↦[struct.t Version] (ver_to_val verLast))%I with "[begin val end]" as "Hver".
+    { iDestruct (struct_fields_split verLastR 1%Qp Version (ver_to_val verLast)
+                  with "[begin end val]") as "Hver"; last iFrame.
+      rewrite /struct_fields.
+      simpl.
+      subst.
+      rewrite u64_Z_through_nat.
+      iFrame.
+      done.
+    }
+    iDestruct ("HversA" with "Hver") as "HversA".
+    iDestruct ("HversL_close" with "[HversA]") as "HversL".
+    { iFrame.
+      iPureIntro.
+      rewrite <- HversLen.
+      apply insert_length.
+    }
+    
+    (* Appending new version. *)
+    wp_pures.
+    wp_loadField.
+    wp_apply (wp_SliceAppend' with "[HversL]").
+    { done. }
+    { auto. }
+    { iFrame. }
+    iIntros (vers') "HversL".
+    wp_apply (wp_storeField with "[Hvers]").
+    { apply slice_val_ty. }
+    { done. }
+    iIntros "Hvers".
+    wp_storeField.
+    wp_storeField.
+    wp_loadField.
+    wp_apply (wp_condBroadcast with "[$HrcondC]").
+    wp_pures.
+    wp_loadField.
+    wp_apply (release_spec with "[-HΦ]").
+    { iFrame "Hlock Hlocked".
+      iNext.
+      iExists (U64 0), tidrd, tid, vers', _.
+      iFrame.
+      iSplitL; last done.
+      instantiate (1:=(<[int.nat (word.sub vers.(Slice.sz) 1):=verLast]> versL) ++ [(tid, (U64 18446744073709551615), val)]).
+      rewrite fmap_app.
+      rewrite list_fmap_insert.
+      iFrame.
+    }
+    wp_pures.
+    iApply "HΦ".
+    done.
+  }
+
+  (* Appending new version (without updating the latest version). *)
+  (***********************************************************)
+  (* verNext := Version{                                     *)
+  (*   begin   : tid,                                        *)
+  (*   end     : config.TID_SENTINEL,                        *)
+  (*   val     : val,                                        *)
+  (* }                                                       *)
+  (* tuple.vers = append(tuple.vers, verNext)                *)
+  (***********************************************************)
+  wp_pures.
+  wp_loadField.
+  wp_apply (wp_SliceAppend' with "[HversL]").
+  { done. }
+  { auto. }
+  { iFrame. }
+  iIntros (vers') "HversL".
+  wp_apply (wp_storeField with "[Hvers]").
+  { apply slice_val_ty. }
+  { done.}
+  iIntros "Hvers".
+  wp_pures.
+
+  (***********************************************************)
+  (* tuple.tidown = 0                                        *)
+  (* tuple.tidwr = tid                                       *)
+  (***********************************************************)
+  wp_storeField.
+  wp_storeField.
+
+  (***********************************************************)
+  (* tuple.rcond.Broadcast()                                 *)
+  (***********************************************************)
+  wp_loadField.
+  wp_apply (wp_condBroadcast with "[$HrcondC]").
+  wp_pures.
+
+  (***********************************************************)
+  (* tuple.latch.Unlock()                                    *)
+  (***********************************************************)
+  wp_loadField.
+  wp_apply (release_spec with "[-HΦ]").
+  { (* Restoring the lock invariant. *)
+    iFrame "Hlock Hlocked".
+    iNext.
+    rewrite /own_tuple.
+    remember (versL ++ [(tid, (U64 18446744073709551615), val)]) as versL'.
+    iExists (U64 0), tidrd, tid, vers', versL'.
+    iFrame.
+    subst.
+    rewrite fmap_app.
+    iFrame.
+  }
+  wp_pures.
+  iApply "HΦ".
+  done.
+Qed.
 
 Lemma val_to_ver_with_val_ty (x : val) :
   val_ty x (uint64T * (uint64T * (uint64T * unitT))%ht) ->
@@ -84,7 +262,7 @@ Local Theorem wp_findRightVer (tid : u64) (vers : Slice.t)
   {{{ slice.is_slice vers (structTy Version) 1 (ver_to_val <$> versL) }}}
     findRightVer #tid (to_val vers)
   {{{ (ver : (u64 * u64 * u64)) (found : bool), RET (ver_to_val ver, #found);
-      ⌜int.Z ver.1.1 ≤ int.Z tid < int.Z ver.1.2⌝ ∗
+      ⌜found = false ∨ (found = true ∧ (int.Z ver.1.1 ≤ int.Z tid < int.Z ver.1.2))⌝ ∗
       slice.is_slice vers (structTy Version) 1 (ver_to_val <$> versL)
   }}}.
 Proof.
@@ -96,7 +274,6 @@ Proof.
   (* var ret Version                                         *)
   (* var found bool = false                                  *)
   (***********************************************************)
-  replace (#0, (#0, (#0, #())))%V with (zero_val (struct.t Version)); last auto.
   wp_apply wp_ref_of_zero; first auto.
   iIntros (verR) "HverR".
   wp_pures.
@@ -112,8 +289,10 @@ Proof.
   (* }                                                       *)
   (***********************************************************)
   wp_apply (slice.wp_forSlice
-              (λ _, (∃ ver : (u64 * u64 * u64), verR ↦[struct.t Version] ver_to_val ver) ∗
-                    (∃ found : bool, foundR ↦[boolT] #found)
+              (λ _, ∃ (ver : u64 * u64 * u64) (found : bool),
+                 (verR ↦[struct.t Version] ver_to_val ver) ∗
+                 (foundR ↦[boolT] #found) ∗
+                 (⌜found = false ∨ (found = true ∧ (int.Z ver.1.1 ≤ int.Z tid < int.Z ver.1.2))⌝)
               )%I
               _ _ _ _ _ (ver_to_val <$> versL)
               with "[] [HverR HfoundR HversL]").
@@ -122,9 +301,9 @@ Proof.
     (* More concise proof here? *)
     iIntros (i x Φ).
     iModIntro.
-    iIntros "([HverR HfoundR] & %Hbound & %Hsome) HΦ".
-    iDestruct "HverR" as (ver) "HverR".
-    iDestruct "HfoundR" as (found) "HfoundR".
+    iIntros "H HΦ".
+    iDestruct "H" as "(H & %Hbound & %Hsome)".
+    iDestruct "H" as (ver found) "(HverR & HfoundR & %Hright)".
     apply val_to_ver_with_lookup in Hsome as (b & e & v & Hx & Hsome).
     subst.
     wp_pures.
@@ -141,38 +320,41 @@ Proof.
       wp_store.
       iApply "HΦ".
       iModIntro.
+      iExists (b, e, v), true.
       iSplitL "HverR"; auto.
     - (* Not the correct version *)
       iApply "HΦ".
       iModIntro.
+      iExists ver, found.
       iSplitL "HverR"; auto.
   }
   { (* Loop invariant holds at the begining *)
     iFrame.
     simpl.
+    iExists ((U64 0), (U64 0), (U64 0)), false.
     iSplitL "HverR"; last auto.
-    iExists ((U64 0), (U64 0), (U64 0)).
     iFrame.
   }
   
   (***********************************************************)
   (*  return ret, found                                      *)
   (***********************************************************)
-  iIntros "[[HverR HfoundR] HversL]".
+  iIntros "[H HversL]".
+  iDestruct "H" as (ver found) "(HverR & HfoundR & %Hright)".
   iDestruct ("HversL_close" with "HversL") as "HversL".
   wp_pures.
-  iDestruct "HverR" as (ver) "HverR".
-  iDestruct "HfoundR" as (found) "HfoundR".
   wp_load.
   wp_load.
   wp_pures.
   iModIntro.
   iApply "HΦ".
   iFrame.
-  (* TODO: Add the relationship between `ver` and `tid` to the loop inv. *)
-  admit.
-Admitted.
+  auto.
+Qed.
 
+(*****************************************************************)
+(* func (tuple *Tuple) ReadVersion(tid uint64) (uint64, bool)    *)
+(*****************************************************************)
 Theorem wp_tuple__ReadVersion tuple_ptr (tid : u64) :
   is_tuple tuple_ptr -∗
   {{{ True }}}
@@ -182,78 +364,101 @@ Proof.
   iIntros "#Htuple !#" (Φ) "_ HΦ".
   iNamed "Htuple".
   wp_call.
+  
+  (***********************************************************)
+  (* tuple.latch.Lock()                                      *)
+  (***********************************************************)
   wp_loadField.
   wp_apply (acquire_spec with "Hlock").
   iIntros "[Hlocked Hown]".
   iNamed "Hown".
   wp_pures.
+
+  (***********************************************************)
+  (* for tid >= tuple.tidwr && tuple.tidown != 0 {           *)
+  (*   tuple.rcond.Wait()                                    *)
+  (* }                                                       *)
+  (***********************************************************)
+  wp_apply (wp_forBreak_cond
+              (λ _,
+                 (own_tuple tuple_ptr latch) ∗
+                 (locked latch))%I
+              with "[] [-HΦ]").
   (**
    * Q: Is it correct to say `wp_forBreak_cond` is used when the loop invariant
    * is the same as the pre/post conditions? Use `wp_apply (wp_forBreak I)` for
    * customized loop invariant?
    *)
-  wp_apply (wp_forBreak_cond'
-              ((own_tuple tuple_ptr latch) ∗
-               (locked latch))
-             with "[-]").
   (* Customize the loop invariant as waiting on condvar havocs the values. *)
-  { iFrame "Hlocked".
+  { (* Loop body preserves the invariant. *)
+    clear Φ.
+    iIntros (Φ).
+    iModIntro.
+    clear tidown tidrd tidwr vers versL.
+    iIntros "[Hown Hlocked] HΦ".
+    iNamed "Hown".
+    wp_pures.
+    wp_loadField.
+    wp_pures.
+    (**
+     * Interesting thing going on here: `wp_and` seems to bind the wrong if.
+     * Reason: Goose generate a similar form for both loops and logical ands.
+     * Solution here is using `wp_bind` to focus on the right if:
+     * `wp_bind (If #(bool_decide _) _ _).`
+     *)
+    wp_bind (If #(bool_decide _) _ _).
+    (* Constructing the condition for blocking readers. *)
+    wp_apply (wp_and with "Htidown").
+    { wp_pures. done. }
+    { iIntros "_ Htidown".
+      wp_loadField.
+      wp_pures.
+      iFrame.
+      iPureIntro.
+      (* Maybe a more concise proof here? *)
+      assert (H : ∀ (P : Prop) (dec : Decision P), negb (bool_decide P) = bool_decide (not P)).
+      { intros P dec. case_bool_decide.
+        - simpl. symmetry. rewrite bool_decide_eq_false. auto.
+        - simpl. symmetry. rewrite bool_decide_eq_true. apply H. }
+      rewrite H.
+      reflexivity.
+    }
+    iIntros "Htidown".
+    wp_if_destruct.
+    { wp_pures.
+      wp_loadField.
+      wp_apply (wp_condWait with "[-HΦ]").
+      { iFrame "Hlock Hlocked HrcondC".
+        iExists tidown, tidrd, tidwr, vers, versL.
+        iFrame "% # ∗".
+      }
+      iIntros "[Hlocked Hown]".
+      wp_pures.
+      iModIntro.
+      iApply "HΦ".
+      iFrame.
+    }
+    iApply "HΦ".
+    iModIntro.
+    iFrame.
     iExists tidown, tidrd, tidwr, vers, versL.
-    iFrame "% ∗". }
-  (* Q: We can intro persistent modality as Hoare triple is persistent? *)
-  iModIntro.
-  clear tidown tidrd tidwr vers versL HversLen.
+    iFrame.
+  }
+  { (* The invariant holds at the start. *)
+    iFrame "Hlocked".
+    iExists tidown, tidrd, tidwr, vers, versL.
+    iFrame "% ∗".
+  }
+  clear tidown tidrd tidwr vers versL.
   iIntros "[Hown Hlocked]".
   iNamed "Hown".
   wp_pures.
-  wp_loadField.
-  wp_pures.
-  (**
-   * Interesting thing going on here: `wp_and` seems to bind the wrong if.
-   * Reason: Goose generate a similar form for both loops and logical ands.
-   * One solution: Use `wp_bind` to focus on the right if.
-   * `wp_bind (If #(bool_decide _) _ _).`
-   * Here we simply destruct `bool_decide c`.
-   *)
-  wp_bind (If #(bool_decide _) _ _).
-  (* Constructing the condition for blocking readers. *)
-  wp_apply (wp_and with "Htidown").
-  { wp_pures. done. }
-  { iIntros "_ Htidown".
-    wp_loadField.
-    wp_pures.
-    iFrame.
-    iPureIntro.
-    (* Maybe a more concise proof here? *)
-    assert (H : ∀ (P : Prop) (dec : Decision P), negb (bool_decide P) = bool_decide (not P)).
-    { intros P dec. case_bool_decide.
-      - simpl. symmetry. rewrite bool_decide_eq_false. auto.
-      - simpl. symmetry. rewrite bool_decide_eq_true. apply H. }
-    rewrite H.
-    reflexivity.
-  }
-  iIntros "Htidown".
-  wp_if_destruct.
-  { (* Loop body preserves the invariant. *)
-    wp_pures.
-    wp_loadField.
-    wp_apply (wp_condWait with "[-]").
-    { iFrame "Hlock Hlocked HrcondC".
-      iExists tidown, tidrd, tidwr, vers, versL.
-      iFrame "% # ∗".
-    }
-    iIntros "[Hlocked Hown]".
-    wp_pures.
-    iModIntro.
-    iLeft.
-    iFrame.
-    done.
-  }
-  (* After the loop. *)
-  iRight.
-  iModIntro.
-  iSplit; first done.
-  wp_pures.
+  
+  (***********************************************************)
+  (* if tuple.tidrd < tid {                                  *)
+  (*   tuple.tidrd = tid                                     *)
+  (* }                                                       *)
+  (***********************************************************)
   wp_loadField.
   wp_pures.
   wp_apply (wp_If_join_evar with "[-]").
@@ -263,7 +468,7 @@ Proof.
       wp_storeField.
       iSplit; first done.
       (* Update "Htidrd" to use `b'` for merging states. See comments of wp_If_join_evar in control.v. *)
-      iAssert (tuple_ptr ↦[Tuple :: "tidrd"] (if b' then #tid else #tidrd)) with "[Htidrd]" as "Htidrd".
+      iAssert (tuple_ptr ↦[Tuple :: "tidrd"] #(if b' then tid else tidrd)) with "[Htidrd]" as "Htidrd".
       { rewrite Eb'. iFrame "Htidrd". }
       iNamedAccu.
     - wp_if_false.
@@ -276,6 +481,64 @@ Proof.
   iNamed "H".
   wp_pures.
 
+  (***********************************************************)
+  (* ver, found := findRightVer(tid, tuple.vers)             *)
+  (***********************************************************)
+  wp_loadField.
+  wp_apply (wp_findRightVer with "HversL").
+  iIntros (ver found) "[%Hright HversL]".
+  wp_pures.
+
+  (***********************************************************)
+  (* if !found {                                             *)
+  (*   tuple.latch.Unlock()                                  *)
+  (*   return 0, false                                       *)
+  (* }                                                       *)
+  (***********************************************************)
+  wp_if_destruct.
+  { wp_loadField.
+    wp_apply (release_spec with "[-HΦ]").
+    { iFrame "Hlock Hlocked".
+      iNext.
+      destruct (bool_decide (int.Z tidrd < int.Z tid)).
+      - iExists tidown, tid, tidwr, vers, versL.
+        iFrame.
+      - iExists tidown, tidrd, tidwr, vers, versL.
+        iFrame.
+    }
+    wp_pures.
+    iModIntro.
+    iApply "HΦ".
+    done.
+  }
+
+  (***********************************************************)
+  (* val := ver.val                                          *)
+  (***********************************************************)
+  wp_pures.
+
+  (***********************************************************)
+  (* tuple.latch.Unlock()                                    *)
+  (***********************************************************)
+  wp_loadField.
+  wp_apply (release_spec with "[-HΦ]").
+  { iFrame "Hlock Hlocked".
+    iNext.
+    destruct (bool_decide (int.Z tidrd < int.Z tid)).
+    - iExists tidown, tid, tidwr, vers, versL.
+      iFrame.
+    - iExists tidown, tidrd, tidwr, vers, versL.
+      iFrame.
+  }
+  wp_pures.
+  iModIntro.
+
+  (***********************************************************)
+  (* return val, true                                        *)
+  (***********************************************************)
+  iApply "HΦ".
+  done.
+
   (**
    * Q1: Can we avoid simplying (zero_val (refT ..)) (to match the form of wp_ref_of_zero)?
    * Q2: How does (zero_val (refT ..)) get simplified when there is no case for refT in zero_val?
@@ -284,9 +547,11 @@ Proof.
   replace #null with (zero_val (refT (struct.t Version))); last first.
   { simpl. reflexivity. }
   *)
-  admit.
-Admitted.
+Qed.
   
+(*****************************************************************)
+(* func (tuple *Tuple) Free(tid uint64)                          *)
+(*****************************************************************)
 Theorem wp_tuple__Free tuple_ptr (tid : u64) :
   is_tuple tuple_ptr -∗
   {{{ True }}}
@@ -296,15 +561,31 @@ Proof.
   iIntros "#Htuple !#" (Φ) "_ HΦ".
   iNamed "Htuple".
   wp_call.
+
+  (***********************************************************)
+  (* tuple.latch.Lock()                                      *)
+  (***********************************************************)
   wp_loadField.
   wp_apply (acquire_spec with "Hlock").
   iIntros "[Hlocked Hown]".
   iNamed "Hown".
   wp_pures.
+
+  (***********************************************************)
+  (* tuple.tidown = 0                                        *)
+  (***********************************************************)
   wp_storeField.
+
+  (***********************************************************)
+  (* tuple.rcond.Broadcast()                                 *)
+  (***********************************************************)
   wp_loadField.
   wp_apply (wp_condBroadcast with "[$HrcondC]").
   wp_pures.
+
+  (***********************************************************)
+  (* tuple.latch.Unlock()                                    *)
+  (***********************************************************)
   wp_loadField.
   wp_apply (release_spec with "[-HΦ]").
   { iFrame "Hlock Hlocked".
@@ -312,124 +593,15 @@ Proof.
     rewrite /own_tuple.
     iExists (U64 0), tidrd, tidwr, vers, versL.
     iFrame.
-    iFrame "#".
-    done.
   }
   wp_pures.
   iApply "HΦ".
   done.
 Qed.
 
-Theorem wp_tuple__AppendVersion tuple_ptr (tid : u64) (val : u64) :
-  is_tuple tuple_ptr -∗
-  {{{ True }}}
-    Tuple__AppendVersion #tuple_ptr #tid #val
-  {{{ b, RET #b; True }}}.
-Proof.
-  iIntros "#Htuple !#" (Φ) "_ HΦ".
-  iNamed "Htuple".
-  unfold Tuple__AppendVersion.
-  wp_pures.
-  wp_loadField.
-  wp_apply (acquire_spec with "Hlock").
-  iIntros "[Hlocked Hown]".
-  iNamed "Hown".
-  wp_pures.
-  wp_loadField.
-  wp_apply wp_slice_len.
-  wp_if_destruct.
-  { (* `vers` not empty *)
-    wp_loadField.
-    wp_apply wp_slice_len.
-    wp_pures.
-    wp_loadField.
-    wp_lam.
-    wp_pures.
-    wp_apply wp_slice_len.
-    
-    wp_if_destruct; last first.
-    { (* prove in-bound *)
-      exfalso.
-      destruct (bool_decide (int.Z vers.(Slice.sz) = int.Z 0)) eqn:E.
-      - apply bool_decide_eq_true in E. lia.
-      - apply bool_decide_eq_false in E.
-        destruct Heqb0.
-        apply word.decrement_nonzero_lt. done.
-    }
-    wp_apply wp_slice_ptr.
-    wp_pures.
-    (* Q: why can't `apply list_lookup_lt.` ? *)
-    (* Below we try to prove the last element of `versL` contains something. *)
-    assert (HversLenLast : ((int.nat (word.sub vers.(Slice.sz) (U64 1))) < length versL)%nat).
-    (* `Set Printing Coercions.` is very helpful here... *)
-    { rewrite HversLen. word. }
-    apply list_lookup_lt in HversLenLast as [x Hsome].
-    iDestruct (big_sepL_delete _ _ (int.nat (word.sub vers.(Slice.sz) 1)) with "Hver") as "[HverLast Hver]".
-    { apply Hsome. }
-    iNamed "HverLast".
-    (* Q: why does wp_storeField not work here? *)
-    wp_apply (wp_storeField with "[Hend]").
-    { auto. }
-    { iModIntro.
-      replace (Z.of_nat (int.nat (word.sub vers.(Slice.sz) 1))) with (1 * int.Z (word.sub vers.(Slice.sz) 1)); last first.
-      { word. }
-      iApply "Hend".
-    }
-    iIntros "Hend".
-
-    (* Appending new version. *)
-    wp_pures.
-    wp_loadField.
-    wp_apply (wp_SliceAppend' with "[HversL]").
-    { done. }
-    { auto. }
-    { iFrame. }
-    iIntros (vers') "HversL".
-    wp_apply (wp_storeField with "[Hvers]").
-    { apply slice_val_ty. }
-    { done. }
-    iIntros "Hvers".
-    wp_storeField.
-    wp_storeField.
-    wp_loadField.
-    wp_apply (wp_condBroadcast with "[$HrcondC]").
-    wp_pures.
-    admit.
-  }
-
-  (* Appending new version (without updating the latest version). *)
-  wp_pures.
-  wp_loadField.
-  wp_apply (wp_SliceAppend' with "[HversL]").
-  { done. }
-  { auto. }
-  { iFrame. }
-  iIntros (vers') "HversL".
-  wp_apply (wp_storeField with "[Hvers]").
-  { apply slice_val_ty. }
-  { done. }
-  iIntros "Hvers".
-  wp_storeField.
-  wp_storeField.
-  wp_loadField.
-  wp_apply (wp_condBroadcast with "[$HrcondC]").
-  wp_pures.
-  wp_loadField.
-  wp_apply (release_spec with "[-HΦ]").
-  { (* Restoring the lock invariant. *)
-    iFrame "Hlock Hlocked".
-    iNext.
-    rewrite /own_tuple.
-    set (versL ++ [(tid, (U64 18446744073709551615), val)]) as versL'.
-    iExists (U64 0), tidrd, tid, vers', versL'.
-    iFrame.
-    admit.
-  }
-  wp_pures.
-  iApply "HΦ".
-  done.
-Admitted.
-  
+(*****************************************************************)
+(* func (tuple *Tuple) Own(tid uint64) bool                      *)
+(*****************************************************************)
 Theorem wp_tuple__Own tuple_ptr (tid : u64) :
   is_tuple tuple_ptr -∗
   {{{ True }}}
@@ -438,20 +610,29 @@ Theorem wp_tuple__Own tuple_ptr (tid : u64) :
 Proof.
   iIntros "#Htuple !#" (Φ) "_ HΦ".
   iNamed "Htuple".
-  unfold Tuple__Own.
-  wp_pures.
+  wp_call.
+  
+  (***********************************************************)
+  (* tuple.latch.Lock()                                      *)
+  (***********************************************************)
   wp_loadField.
   wp_apply (acquire_spec with "Hlock").
   iIntros "[Hlocked Hown]".
   iNamed "Hown".
   wp_pures.
+
+  (***********************************************************)
+  (* if tid < tuple.tidrd || tid < tuple.tidwr {             *)
+  (*   tuple.latch.Unlock()                                  *)
+  (*   return false                                          *)
+  (* }                                                       *)
+  (***********************************************************)
   wp_loadField.
   wp_apply (wp_or with "[Htidwr]").
   { iApply "Htidwr". }
   { wp_pures. done. }
   { iIntros "_ Hidwr". wp_loadField. wp_pures. iFrame. done. }
   iIntros "Hidrwr".
-  (* Branch on `tid < tuple.tidrd` *)
   wp_if_destruct.
   { (* Early return: `tid < tuple.tidrd || tid < tuple.tidwr` *)
     wp_loadField.
@@ -460,14 +641,18 @@ Proof.
       iNext.
       iExists tidown, tidrd, tidwr, vers, versL.
       iFrame.
-      done.
     }
     wp_pures.
     iModIntro. iApply "HΦ". done.
   }
-  (* `!(tid < tuple.tidrd || tid < tuple.tidwr)` *)
+
+  (***********************************************************)
+  (* if tuple.tidown != 0 {                                  *)
+  (*   tuple.latch.Unlock()                                  *)
+  (*   return false                                          *)
+  (* }                                                       *)
+  (***********************************************************)
   wp_loadField.
-  (* Branch on `tuple.tidown != 0` *)
   wp_if_destruct.
   { (* Early return: `tuple.tidown != 0` *)
     wp_loadField.
@@ -476,23 +661,32 @@ Proof.
       iNext.
       iExists tidown, tidrd, tidwr, vers, versL.
       iFrame.
-      done.
     }
     wp_pures.
     iModIntro. iApply "HΦ". done.
   }
-  (* `!(tuple.tidown != 0)` *)
+
+  (***********************************************************)
+  (* tuple.tidown = tid                                      *)
+  (***********************************************************)
   wp_storeField.
+
+  (***********************************************************)
+  (* tuple.latch.Unlock()                                    *)
+  (***********************************************************)
   wp_loadField.
   wp_apply (release_spec with "[-HΦ]").
   { iFrame "Hlock Hlocked".
     iNext.
     iExists tid, tidrd, tidwr, vers, versL.
     iFrame.
-    done.
   }
   wp_pures.
   iModIntro.
+
+  (***********************************************************)
+  (* return true                                             *)
+  (***********************************************************)
   iApply "HΦ".
   done.
 Qed.
